Test/dafny0/SplitExpr.dfy
@@ -1,0 +1,56 @@
+class UnboundedStack<T> {
+  var top: Node<T>;
+  ghost var footprint: set<object>;
+  ghost var content: seq<T>; 
+
+  function IsUnboundedStack(): bool
+    reads {this} + footprint;
+  {
+    this in footprint &&
+    (top == null  ==>  content == []) &&
+    (top != null  ==>  top in footprint && top.footprint <= footprint &&
+                       top.prev == null && content == top.content && top.Valid())
+  }
+
+  function IsEmpty(): bool
+    reads {this};
+  { content == [] }
+
+  method Pop() returns (result: T)
+    requires IsUnboundedStack() && !IsEmpty();
+    modifies footprint;
+    ensures IsUnboundedStack() && content == old(content)[1..];
+  {
+    result := top.val;
+    // The following assert does the trick, because it gets inlined and thus
+    // exposes top.next.Valid() (if top.next != null):
+    footprint := footprint - top.footprint;  top := top.next;
+    // In a previous version of the implementation of the SplitExpr transformation, the
+    // following assert did not have the intended effect of being used as a lemma:
+    assert top != null ==> top.Valid();
+    if (top != null) {
+      footprint := footprint + top.footprint;  top.prev := null;
+    }
+    content := content[1..];
+} }
+
+class Node<T> {
+  var val: T;  
+  var next: Node<T>;
+  var prev: Node<T>;
+  var footprint: set<Node<T>>;
+  var content: seq<T>;
+
+  function Valid(): bool
+    reads this, footprint;
+  {
+    this in footprint && !(null in footprint) &&
+    (next == null  ==>  content == [val])  &&
+    (next != null  ==>  next in footprint &&
+                        next.footprint < footprint &&
+                        !(this in next.footprint) &&
+                        next.prev == this &&
+                        content == [val] + next.content &&
+                        next.Valid())
+  }
+}
